Hoare/Hoare_Step.thy
@@ -278,8 +278,267 @@ proof(rule HT'I)
     by blast
 qed
 
-(* TODO: there is a spurious Pord constraint on f for some reason. *)
+
 lemma HTS_imp_HT'' :
+  fixes f :: "'syn0 \<Rightarrow> 'st0 \<Rightarrow> 'st0"
+  fixes x :: "'syn1"
+  fixes l' :: "('syn1 \<Rightarrow> 'syn0)"
+  assumes H: "f % {{P'}} (l' x) {{Q'}}"
+  assumes Valid : "lifting_validx l S"
+  assumes Hf' : "f' = lift_map_s l' (no_control_lifting  l) f"
+  assumes H0 : "gs = pcomps fs"
+  assumes Hpres : "sups_pres (set fs)"
+  assumes Hseq : "seq_sem_l_gen lfts \<in> set fs"
+  assumes Skip : "lfts x = Sskip"
+  assumes Hnemp : "g \<in> (set fs - {seq_sem_l_gen lfts})"
+  assumes Hdom : "(f' \<downharpoonleft> (set fs - {seq_sem_l_gen lfts}) x)"
+  assumes P1_ok : "\<And> st . P st \<Longrightarrow> st \<in> ok_S"
+  assumes HP : "\<And> st . P st \<Longrightarrow> P' (LOut l (l' x) st)"
+
+  shows "|gs| {~ (\<lambda> st . P st) ~} [G x z] 
+    {~ (\<lambda> st . \<exists> old_big small_new . P old_big \<and> Q' small_new \<and> st = LUpd l (l' x) small_new old_big) ~}"
+  (*shows "\<And> P1 . |gs| {~ P1 ~} [G c z] {~ (liftt_conc id l c P2 P1) ~}"*)
+proof(rule HT'I)
+  term "l'"
+  term "gs"
+  fix npost
+  have Valid' : "lifting_valid l S"
+    using lifting_validxDV[OF Valid] by auto
+
+  have "|#gs#| {#-(\<lambda>st. P st), (0 + npost)-#} [G x z] {#-(\<lambda>st. \<exists>old_big small_new.
+            P old_big \<and>
+            Q' small_new \<and>
+            st = LUpd l (l' x)  small_new old_big), npost-#}"
+    unfolding add_0
+  proof
+    fix c'
+
+    assume Guard : " |#gs#| {#(\<lambda>st. \<exists>old_big small_new.
+                            P old_big \<and>
+                            Q' small_new \<and>
+                            st =
+                            LUpd l (l' x) small_new
+                             old_big), npost#} c'"
+    show "|#gs#| {#P, npost#} ([G x z] @ c')"
+    proof
+      fix m 
+      assume Hpay0 : "P (payload m)" and Hcont : "cont m = Inl ([G x z] @ c') "
+
+      show "safe_for gs m npost"
+      proof(cases "(sem_step gs m)")
+        case (Inr bad)
+  
+        then have False using Hcont H0
+          by(auto simp add: sem_step_def)
+  
+        then show ?thesis by auto
+      next
+        case (Inl m')
+
+        have Pres' : "sups_pres (set fs - {seq_sem_l_gen lfts})"
+          using sups_pres_subset[OF Hpres, of "set fs - {seq_sem_l_gen lfts}"] by auto
+
+        obtain fs_sub where Fs_sub : "set fs_sub = set fs - {seq_sem_l_gen lfts}"
+          using finite_list[of "set fs - {seq_sem_l_gen lfts}"]
+          by auto
+
+(* ok, so the idea now is:
+- we know full step (op + control flow) leads to m'
+- dominance over everything but the seq means we can treat it as
+  "op (dominant thing) then seq"
+- we can then unfold these things in order and everything should be ok.
+*)
+
+        have Assoc : 
+             "pcomps (fs_sub @ [seq_sem_l_gen lfts]) =
+              pcomps [pcomps fs_sub, pcomps [seq_sem_l_gen lfts]]"
+        proof(rule pcomps_assoc)
+
+          have "set fs - {seq_sem_l_gen lfts} \<union> set [seq_sem_l_gen lfts] = set fs"
+            using Hseq 
+            by(simp; blast)
+
+          then show "sups_pres (set fs_sub \<union> set [seq_sem_l_gen lfts])"
+            unfolding Fs_sub
+            using Hpres
+            by auto
+        next
+
+          have "set fs_sub \<noteq> {}" using Hnemp unfolding Fs_sub by auto
+
+          then show "fs_sub \<noteq> []" by auto
+        next
+
+          show "[seq_sem_l_gen lfts] \<noteq> []" by simp
+        qed
+
+        have Set_alt : "set (fs_sub @ [seq_sem_l_gen lfts]) = set fs"
+          unfolding set_append Fs_sub
+          using Un_Diff_cancel2 Hseq
+          by auto
+
+        have Gs_alt : "gs = pcomps (fs_sub @ [seq_sem_l_gen lfts])"
+          using pcomps_set_eq[OF Hpres Hseq _ Set_alt, of fs] H0
+          by auto
+
+
+        have Hpay : "P (payload m)"
+          using Hpay0
+          by auto
+
+        then have Hpay_S : "payload m \<in> ok_S"
+          using P1_ok[of "payload m"] by auto
+
+        have Hpay1' : "LOut l (l' x) (payload m) = LOut l (l' x) (payload m) \<and> P (payload m)"
+          using Hpay
+          by simp
+
+      have Hpay' : "Q' (f (l' x) (LOut l (l' x) (payload m)))"
+        using HTSE[OF H ] HP[OF Hpay]
+        by auto
+
+  (*
+        then have Hpay1 : "\<exists>full. LOut l (id c) full = LOut l c (payload m) \<and> P1 full" using Hpay_S
+          by auto
+
+        have Hpay' : " P2 (\<lambda>st. \<exists>full. LOut l (id c) full = st \<and> P1 full) (f c (LOut l c (payload m)))"
+          using HTSE[OF H ] Hpay1
+          by auto
+*)
+(* TODO: find a better solution than this awful type annotation hack *)
+
+        have Seq_pres : 
+          "sups_pres {(seq_sem_l_gen lfts  ::('syn1 \<Rightarrow> 'syn1 gensyn list md_triv option md_prio \<times>
+            String.literal md_triv option md_prio \<times> 'a
+            \<Rightarrow> 'syn1 gensyn list md_triv option md_prio \<times>
+               String.literal md_triv option md_prio \<times>
+               'a))}"
+          using sups_pres_subset[OF Hpres, of "{(seq_sem_l_gen lfts )}"] Hseq
+          by(auto)
+
+        have Gs_alt' : "gs = pcomps [pcomps fs_sub, seq_sem_l_gen lfts]"
+          using Gs_alt pcomps_singleton[OF Seq_pres, of "[seq_sem_l_gen lfts]"]
+          unfolding Assoc
+          unfolding append.simps H0
+          by auto
+
+        have Hdom' :  "f' \<downharpoonleft> (set fs_sub) x"
+          using Fs_sub Hdom by auto
+
+        have Dominate1 : "pcomps fs_sub x m = f' x m" using dominant_pcomps[OF _ _ Hdom', of g m] Pres' Hnemp Fs_sub
+          by auto
+
+(* YOU ARE HERE. *)
+(* problem: seems like we still need to know something about the validity of the initial state.
+   maybe this is OK, but i worry that it will create problems.
+   the obvious solution is just to throw the validity condition into the pre and post conditions.
+   but let's think about whether that will have unintended consequences.
+ *)
+        obtain pri1 pri2 rest where Msplit :
+          "m = (mdp pri1 (Some (mdt (G x z # c'))), mdp pri2 None, rest)" and Rest : "rest \<in> ok_S"
+          using Gs_alt' Dominate1 Skip Hpay Hcont Hf' Hpay_S
+          by(auto simp add: seq_sem_l_gen_def seq_sem_lifting_gen_def 
+            lift_pred_valid_s_def lift_pred_validx_s_def lift_pred_s_def
+            no_control_lifting_def cont_def
+            schem_lift_defs fst_l_def snd_l_def prio_l_def triv_l_def option_l_def seq_sem_def
+            prod_bsup no_control_l_def
+            split: md_prio.splits prod.splits md_triv.splits option.splits list.split_asm)
+
+        have Rest' : "rest \<in> S (l' x)"
+          using lifting_validxDS[OF Valid] Rest by auto
+
+        have LUpd_rest1 :
+          "rest <[ LUpd l (l' x) (f (l' x) (LOut l (l' x) rest)) rest"
+          using lifting_validDI[OF Valid' Rest']
+          by auto
+
+        have LUpd_rest2 : "[^ LUpd l (l' x) (f (l' x) (LOut l (l' x) rest)) rest, rest ^] = LUpd l (l' x) (f (l' x) (LOut l (l' x) rest)) rest"
+          using bsup_base_leq2[OF LUpd_rest1]
+          by simp
+
+        then have LOut_m : 
+          "LOut (l_synt l' (no_control_lifting l)) x (gs x m) = LOut (l_synt l' (no_control_lifting l)) x (f' x m)"
+          using Gs_alt' Dominate1 Skip Hpay Hcont Hf' Msplit
+          unfolding l_synt_def
+          by(auto simp add: seq_sem_l_gen_def seq_sem_lifting_gen_def 
+            lift_pred_valid_s_def lift_pred_s_def
+            no_control_lifting_def cont_def
+            schem_lift_defs fst_l_def snd_l_def prio_l_def triv_l_def option_l_def seq_sem_def
+            prod_bsup no_control_l_def
+            split: md_prio.splits prod.splits md_triv.splits option.splits list.split_asm)
+
+
+(* key sub-result. *)
+
+(* key sub-result. idea here is that no_control_l means we won't overwrite. *)
+        have Cont_final : "cont m' = cont (seq_sem_l_gen lfts x m)"
+          using Hcont Msplit Skip Inl Gs_alt' Dominate1 Hf'
+          by(auto simp add: seq_sem_l_gen_def seq_sem_lifting_gen_def sem_step_def
+            lift_pred_valid_s_def lift_pred_s_def
+            no_control_lifting_def cont_def
+            schem_lift_defs fst_l_def snd_l_def prio_l_def triv_l_def option_l_def seq_sem_def
+            prod_bsup no_control_l_def prio_bsup option_bsup leq_refl
+            split: md_prio.splits prod.splits md_triv.splits option.splits list.split_asm)         
+
+        hence Cont_final' : "cont m' = Inl c'"
+          using Hcont Msplit Skip
+          by(auto simp add: seq_sem_l_gen_def seq_sem_lifting_gen_def sem_step_def
+            lift_pred_valid_s_def lift_pred_s_def
+            no_control_lifting_def cont_def
+            schem_lift_defs fst_l_def snd_l_def prio_l_def triv_l_def option_l_def seq_sem_def
+            prod_bsup no_control_l_def
+            split: md_prio.splits prod.splits md_triv.splits option.splits list.split_asm)
+
+        have Pay_final : "payload m' = LUpd l (l' x) (f (l' x) (LOut l (l' x) (payload m))) (payload m)"
+          using Gs_alt' Dominate1 Skip Hpay Hcont Hf' Msplit Inl LUpd_rest2
+          by(auto simp add: seq_sem_l_gen_def seq_sem_lifting_gen_def sem_step_def
+            lift_pred_valid_s_def lift_pred_s_def
+            no_control_lifting_def cont_def
+            schem_lift_defs fst_l_def snd_l_def prio_l_def triv_l_def option_l_def seq_sem_def
+            prod_bsup no_control_l_def
+            split: md_prio.splits prod.splits md_triv.splits option.splits list.split_asm)
+
+(* YOU ARE HERE *)
+(* TODO: we need to pull out the "ok_S" piece. *)
+        have "(P (payload m)) \<and> Q' ((f (l' x) (LOut l (l' x) (payload m)))) \<and>
+              payload m' = LUpd l (l' x) (f (l' x) (LOut l (l' x) (payload m)))(payload m)"
+          using Hpay' Pay_final Hpay_S Hpay
+          by(auto)
+
+        then have Guard_Hyp : "\<exists>old_big small_new.
+             P old_big \<and>
+             Q' small_new \<and>
+             payload m' = LUpd l (l' x) small_new old_big"
+          by auto
+
+        have Conc' : "safe_for gs m' npost"
+          using guardediD[OF Guard, of "m'"]  Cont_final' Guard_Hyp 
+          unfolding Pay_final Cont_final' lift_pred_valid_s_def lift_pred_s_def lift_pred_validx_s_def
+            liftt_conc_def
+          using lifting_validDO[OF Valid'] lifting_validDP[OF Valid'] lifting_validxDP'[OF Valid ]
+          by(cases m; auto)
+
+        have Inl_alt : "sem_step_p gs m m'"
+          using Inl unfolding sem_step_p_eq by simp
+
+        show  "safe_for gs m npost"
+          using safe_for_weaken[OF safe_for_extend[OF Conc' Excp_1[OF Inl_alt]], of npost]
+          by simp
+      qed
+    qed
+  qed
+
+  thus "\<exists>npre.
+          |#gs#| {#-P, (npre +
+                        npost)-#} [G x
+  z] {#-(\<lambda>st. \<exists>old_big small_new.
+                  P old_big \<and>
+                  Q' small_new \<and>
+                  st = LUpd l (l' x) small_new old_big), npost-#}"
+    by blast
+qed
+
+lemma HTS_imp_HT''old :
   assumes H: "\<And> P1 . f % {{P1}} c {{P2 P1}}"
   assumes Valid : "lifting_validx l S"
   assumes Hf' : "f' = no_control_l l f"
